\documentclass[12pt]{report}
\usepackage[utf8]{inputenc}
\begin{document}

\section*{Task}

Perform $\beta$ - reduction of $\lambda$ - term $((\lambda a.(\lambda b.b\; b)\; (\lambda b.b\; b))\; b)\; ((\lambda c.(c\; b))\; (\lambda a.a))$ \newline

\section*{Solution}

$$((\lambda a.(\lambda b.b\; b)\; (\lambda b.b\; b))\; b)\; ((\lambda c.(c\; b))\; (\lambda a.a)) \rightarrow_\beta$$

$$((\lambda a.(\lambda b.b\; b)\; (\lambda b.b\; b))\; b)\; ((\lambda a.a)\; b)) \rightarrow_\beta$$

$$((\lambda a.(\lambda b.b\; b)\; (\lambda b.b\; b))\; b)\; b \rightarrow_\beta$$

$$((\lambda b.b\; b)\; (\lambda b.b\; b))\; b$$

\end{document}