\documentclass[12pt]{report}
\usepackage[utf8]{inputenc}
\begin{document}

\section*{Task}

Prove that $S K K = I$ \newline

\section*{Solution}

$$S = \lambda x\; y\; z.x\; z\; (y\; z)$$

$$K = \lambda x\; y.x$$

$$I = \lambda x.x$$

$$S K K = (S K) K \rightarrow_\beta$$

$$((\lambda x\; y\; z.x\; z\; (y\; z))\; K\; K\rightarrow_\beta$$

$$((\lambda y\; z.K z\; (y\; z))\; K\rightarrow_\beta$$

$$((\lambda z.K z\; (K z))\rightarrow_\beta$$

$$((\lambda z.K z\; (K z))\rightarrow_\beta$$

$$(\lambda z.z)\rightarrow_\beta$$

$$I$$

\end{document}